Progress in CCP proofs

proof/CCP/TypeCase.v
@@ -2,14 +2,182 @@ Require Import Termes.
 Require Import Reduction.
 Require Import Conv.
 Require Import LiftSubst.
-Require Import CCSum.Types.
-Require Import CCSum.Inversion.
-Require Import CCSum.Thinning.
-Require Import CCSum.Substitution.
+Require Import Env.
+Require Import CCP.Types.
+Require Import CCP.Coercion.
+Require Import CCP.Inversion.
+Require Import CCP.Thinning.
+Require Import CCP.Substitution.
 
 Implicit Types i k m n p : nat.
 Implicit Type s : sort.
 Implicit Types A B M N T t u v : term.
+Implicit Types e f g : env.
+
+Definition is_redex (t : term) := 
+match t with 
+| (App (Abs _ _) _) => True
+| _ => False
+end.
+
+Lemma is_redex_dec : forall t, is_redex t \/ ~ is_redex t.
+Proof.
+intros.
+induction t  ; simpl ;  auto.
+induction t1 ; simpl ; auto.
+Qed.
+
+Lemma is_redex_lemma: 
+  forall t : term, is_redex t -> exists M, exists U, exists V, t = App (Abs M U) V.
+Proof.
+intros.
+induction t ; simpl ; simpl in H ; auto ; intuition.
+induction t1 ; simpl ; simpl in H ; auto ; intuition.
+exists t1_1 ; exists t1_2 ; exists t2 ; auto.
+Qed.
+
+
+Inductive hnf : term -> term -> Prop :=
+  | hnf_beta : forall T M U U', hnf (subst T U) U' ->  hnf (App (Abs M U) T) U'
+  | hnf_other : forall T, ~ is_redex T -> hnf T T.
+
+Lemma hnf_injection : forall t, exists t', hnf t t'.
+Proof.
+intros. 
+set (tfull := t).
+induction t ; auto with coc core ; try solve [exists tfull ; apply hnf_other ; unfold tfull ; red ; auto].
+unfold tfull.
+induction t1 ; simpl ; auto with coc core ; try solve [exists tfull ; apply hnf_other ; unfold tfull ; red ; auto].
+exists (subst 
+
+induction (is_redex_lemma t H).
+induction H0.
+induction H0.
+exists (
+
+
+
+Lemma hnf_conv : forall t t', hnf t t' -> conv t t'.
+intros.
+induction H.
+apply trans_conv_conv with (subst T U) ; auto with coc core.
+apply refl_conv.
+Qed.
+
+Definition is_subset (t : term) := 
+match t with 
+| (Subset _ _) => True
+| _ => False
+end.
+
+Definition is_subset_dec (t : term) := 
+match t with 
+| (Subset _ _) => true
+| _ => false
+end.
+
+Lemma is_subset_lemma : forall t : term, is_subset t \/ ~is_subset t.
+Proof.
+intros.
+induction t ; simpl ; auto.
+Qed.
+
+Lemma is_subset_impl: forall t : term, is_subset t -> exists U, exists V, t = Subset U V.
+Proof.
+intros.
+induction t ; simpl ; simpl in H ; auto ; intuition.
+exists t1 ; exists t2 ; auto.
+Qed.
+
+Inductive mu : term -> term -> Prop :=
+| mu_subset : forall T U P, hnf T (Subset U P) ->  
+forall U', mu U U' -> mu T U'
+
+   | mu_other : forall T T',  hnf T T' -> 
+   ~ (exists U, exists P, T' = (Subset U P)) ->
+   mu T T.
+
+Fixpoint mu_rec (t : term) (hnf : term -> term) { struct t }: term :=
+  match t with
+    Subset U P => mu_rec U hnf
+    | _ => t
+ end.
+
+Lemma inv_coerce_prod : forall S T, S >> T -> forall A B, S = (Prod A B) ->
+  forall T', mu T T' -> 
+  exists A', exists B', conv T' (Prod A' B').
+Proof.
+intros S T H; induction H ; intros ; try rewrite H0 in H ; auto with coc core ; 
+try discriminate.
+
+
+inversion H1.
+pose (trans_conv_conv _ B (Subset U P) H (hnf_conv _ _ H2)).
+elim (conv_prod_subset _ _ _ _ c).
+
+rewrite H5 in H ; auto with coc.
+exists A0 ; exists B0 ; auto with coc.
+
+inversion H2.
+pose (hnf_conv _ _ H3).
+elim conv_prod_subset with A' B' U P ; auto with coc core.
+
+exists A' ; exists B' ; auto with coc.
+
+inversion H1.
+inversion H2.
+rewrite <- H6 in H3.
+apply (IHcoerce _ _ H0 T' H3).
+
+inversion H2.
+elim H3.
+exists U' ; exists P ; auto with coc.
+
+induction (is_subset_lemma B).
+induction (is_subset_impl _ H3).
+induction H4.
+cut(exists x', mu x x').
+
+pose (IHcoerce1 A0 B0 H1).
+
+
+Lemma inv_typ_sort_set : forall G t, G |- t : (Srt set) -> ~ conv t (Srt set).
+Proof.
+intros.
+red ; intros.
+inversion H0.
+rewrite H1 in H.
+pose (inv_typ_set G (Srt set) H).
+inversion c.
+apply conv_kind_set ; auto with coc core.
+Admitted.
+
+
+
+Lemma subset_inv : forall G U P T, G |- Subset U P : T ->
+  forall s, ~ conv U (Srt s).
+Proof.
+intros G U P T typUP.
+apply inv_typ_subset with G U P T ; auto.
+intros.
+red ; intros.
+Admitted.
+
+Lemma coerce_sorts : forall G t1 t2 s, G |- t1 : (Srt s) -> G |- t2 : Srt s -> t1 >> t2 ->
+  (forall s1, t1 = Srt s1 -> conv t2 (Srt s1)) /\ (forall s2, t2 = Srt s2 -> conv t1 (Srt s2)).
+Proof.
+  intros.
+  induction H1 ; try (split ; intros ; discriminate).
+  split ; intros ; auto with coc ; try rewrite <- H2 ; auto with coc.
+
+  split ; intros.
+  discriminate.
+  induction IHcoerce.
+  pose (H4 _ H2).
+  
+  apply inv_typ_subset with G U P (Srt s) ; auto with coc core.
+  intros.
+  
 
   Theorem type_case :
    forall e t T,
