proof/CCP/Substitution.v
@@ -1,13 +1,16 @@
 Require Import Termes.
 Require Import Reduction.
 Require Import LiftSubst.
-Require Import CCSum.Types.
-Require Import CCSum.Inversion.
-Require Import CCSum.Thinning.
+Require Import Env.
+Require Import CCP.Types.
+Require Import CCP.Coercion.
+Require Import CCP.Inversion.
+Require Import CCP.Thinning.
 
 Implicit Types i k m n p : nat.
 Implicit Type s : sort.
 Implicit Types A B M N T t u v : term.
+Implicit Types e f g : env.
 
   Lemma wf_sort_lift :
    forall n e t, wf e -> item_lift t e n -> exists s : sort, typ e t (Srt s).
@@ -44,71 +47,6 @@ exists x; auto with coc core arith datatypes.
 inversion_clear H3.
 apply typ_wf with y (Srt s); auto with coc core arith datatypes.
 Qed.
-
-
-
-  Inductive sub_in_env t T : nat -> env -> env -> Prop :=
-    | sub_O : forall e, sub_in_env t T 0 (T :: e) e
-    | sub_S :
-        forall e f n u,
-        sub_in_env t T n e f ->
-        sub_in_env t T (S n) (u :: e) (subst_rec t u n :: f).
-
-  Hint Resolve sub_O sub_S: coc.
-
-  Lemma nth_sub_sup :
-   forall t T n e f,
-   sub_in_env t T n e f ->
-   forall v : nat, n <= v -> forall u, item _ u e (S v) -> item _ u f v.
-simple induction 1.
-intros.
-inversion_clear H1; auto with coc core arith datatypes.
-
-simple destruct v; intros.
-inversion_clear H2.
-
-inversion_clear H3; auto with coc core arith datatypes.
-Qed.
-
-
-  Lemma nth_sub_eq : forall t T n e f, sub_in_env t T n e f -> item _ T e n.
-simple induction 1; auto with coc core arith datatypes.
-Qed.
-
-
-  Lemma nth_sub_inf :
-   forall t T n e f,
-   sub_in_env t T n e f ->
-   forall v : nat,
-   n > v -> forall u, item_lift u e v -> item_lift (subst_rec t u n) f v.
-simple induction 1.
-intros.
-inversion_clear H0.
-
-simple destruct v; intros.
-elim H3; intros.
-rewrite H4.
-inversion_clear H5.
-exists (subst_rec t u n0); auto with coc core arith datatypes.
-apply commut_lift_subst; auto with coc core arith datatypes.
-
-elim H3; intros.
-rewrite H4.
-inversion_clear H5.
-elim H1 with n1 (lift (S n1) x); intros; auto with coc core arith datatypes.
-exists x0; auto with coc core arith datatypes.
-rewrite simpl_lift; auto with coc core arith datatypes.
-pattern (lift (S (S n1)) x0) in |- *.
-rewrite simpl_lift; auto with coc core arith datatypes.
-elim H5.
-change
-  (subst_rec t (lift 1 (lift (S n1) x)) (S n0) =
-   lift 1 (subst_rec t (lift (S n1) x) n0)) in |- *.
-apply commut_lift_subst; auto with coc core arith datatypes.
-
-exists x; auto with coc core arith datatypes.
-Qed.
-
 
   Lemma typ_sub_weak :
    forall g (d : term) t,
@@ -186,6 +124,7 @@ apply type_let_in with (subst_rec d U0 n) s1 s2 ; auto with coc core arith datat
 apply wf_var with s1 ; auto with coc core arith datatypes.
 
 apply type_conv with (subst_rec d U0 n) s; auto with coc core arith datatypes.
+apply coerce_subst_rec ; auto with coc core.
 Qed.
 
   Theorem substitution :
